<?xml version="1.0"?>
<rdf:RDF xmlns="http://www.ease-crc.org/ont/cram_tasks.owl#"
     xml:base="http://www.ease-crc.org/ont/cram_tasks.owl"
     xmlns:owl="http://www.w3.org/2002/07/owl#"
     xmlns:rdf="http://www.w3.org/1999/02/22-rdf-syntax-ns#"
     xmlns:xml="http://www.w3.org/XML/1998/namespace"
     xmlns:xsd="http://www.w3.org/2001/XMLSchema#"
     xmlns:rdfs="http://www.w3.org/2000/01/rdf-schema#"
     xmlns:soma="http://www.ease-crc.org/ont/SOMA#">
    <owl:Ontology rdf:about="http://www.ease-crc.org/ont/cram_tasks.owl">
        <owl:imports rdf:resource="http://www.ease-crc.org/ont/SOMA-ACT.owl"/>
        <owl:imports rdf:resource="http://www.ontologydesignpatterns.org/ont/dul/DUL.owl"/>
    </owl:Ontology>
    


    <!-- 
    ///////////////////////////////////////////////////////////////////////////////////////
    //
    // Classes
    //
    ///////////////////////////////////////////////////////////////////////////////////////
     -->

    


    <!-- http://www.ease-crc.org/ont/SOMA#GetTaskParameter -->

    <owl:Class rdf:about="http://www.ease-crc.org/ont/SOMA#GetTaskParameter"/>
    


    <!-- http://www.ease-crc.org/ont/cram_tasks.owl#GetActionGrasps -->

    <owl:Class rdf:about="http://www.ease-crc.org/ont/cram_tasks.owl#GetActionGrasps">
        <rdfs:subClassOf rdf:resource="http://www.ease-crc.org/ont/SOMA#GetTaskParameter"/>
        <rdfs:comment>Retrieve grasp poses for a manipulation action.</rdfs:comment>
    </owl:Class>
    


    <!-- http://www.ease-crc.org/ont/cram_tasks.owl#GetActionGripperOpening -->

    <owl:Class rdf:about="http://www.ease-crc.org/ont/cram_tasks.owl#GetActionGripperOpening">
        <rdfs:subClassOf rdf:resource="http://www.ease-crc.org/ont/SOMA#GetTaskParameter"/>
        <rdfs:comment>Retrieve gripper opening for a manipulation action performed with a pincer-type gripper.</rdfs:comment>
    </owl:Class>
    


    <!-- http://www.ease-crc.org/ont/cram_tasks.owl#GetActionGrippingEffort -->

    <owl:Class rdf:about="http://www.ease-crc.org/ont/cram_tasks.owl#GetActionGrippingEffort">
        <rdfs:subClassOf rdf:resource="http://www.ease-crc.org/ont/SOMA#GetTaskParameter"/>
        <rdfs:comment>Retrieve grasping force for a manipulation action.</rdfs:comment>
    </owl:Class>
    


    <!-- http://www.ease-crc.org/ont/cram_tasks.owl#GetActionTrajectory -->

    <owl:Class rdf:about="http://www.ease-crc.org/ont/cram_tasks.owl#GetActionTrajectory">
        <rdfs:subClassOf rdf:resource="http://www.ease-crc.org/ont/SOMA#GetTaskParameter"/>
        <rdfs:comment>Retrieve motion trajectory for a (usually manipulation) action.</rdfs:comment>
    </owl:Class>
    


    <!-- http://www.ease-crc.org/ont/cram_tasks.owl#GetContainerClosingDistance -->

    <owl:Class rdf:about="http://www.ease-crc.org/ont/cram_tasks.owl#GetContainerClosingDistance">
        <rdfs:subClassOf rdf:resource="http://www.ease-crc.org/ont/SOMA#GetTaskParameter"/>
        <rdfs:comment>Retrieve a distance parameter used to close a container; e.g., how much to push a drawer before it closes would depend on how pulled out it is.</rdfs:comment>
    </owl:Class>
    


    <!-- http://www.ease-crc.org/ont/cram_tasks.owl#GetContainerOpeningDistance -->

    <owl:Class rdf:about="http://www.ease-crc.org/ont/cram_tasks.owl#GetContainerOpeningDistance">
        <rdfs:subClassOf rdf:resource="http://www.ease-crc.org/ont/SOMA#GetTaskParameter"/>
        <rdfs:comment>Retrieve a distance parameter used to open a container; e.g., how much to pull out a drawer such that its typical contents can be easily accessed and removed.</rdfs:comment>
    </owl:Class>
    


    <!-- http://www.ease-crc.org/ont/cram_tasks.owl#GetLocationPoses -->

    <owl:Class rdf:about="http://www.ease-crc.org/ont/cram_tasks.owl#GetLocationPoses">
        <rdfs:subClassOf rdf:resource="http://www.ease-crc.org/ont/SOMA#GetTaskParameter"/>
        <rdfs:comment>Retrieve poses for a manipulation action.</rdfs:comment>
    </owl:Class>
</rdf:RDF>



<!-- Generated by the OWL API (version 4.5.9.2019-02-01T07:24:44Z) https://github.com/owlcs/owlapi -->

